txn-data-consistency/Closedness.thy
@@ -1,99 +1,158 @@
 theory Closedness
-  imports CCv_Eiger_Port_plus
+  imports Main
 begin
 
-section \<open>General lemmas about the closedness\<close>
-definition closed_general :: "'txn set \<Rightarrow> 'txn rel \<Rightarrow> 'txn set \<Rightarrow> bool" where
-  "closed_general vis r r_only \<equiv> vis = ((r\<^sup>*) `` (vis)) - r_only"
+section \<open>Lemmas about relational image and transititve closure\<close>
 
-lemma closed'_generalize: "closed' K u r = closed_general (visTx' K u) (r^-1) (read_only_Txs K)"
-  by (simp add: closed'_def closed_general_def rtrancl_converse)
+lemma L1: "x \<notin> (r\<^sup>*) `` V \<Longrightarrow> ({z. (z, x) \<in> r\<^sup>*} \<times> B) `` V = {}"
+  by auto
 
-\<comment> \<open>union read version + deps\<close>
-lemma union_closed_general:
-  assumes "closed_general vis\<^sub>1 r r_only"
-      and "closed_general vis\<^sub>2 r r_only"
-      and "r_only \<subseteq> r_only'"
-      and "(r_only' - r_only) \<inter> (vis\<^sub>1 \<union> vis\<^sub>2) = {}"
-    shows "closed_general (vis\<^sub>1 \<union> vis\<^sub>2) r r_only'"
+lemma Image_trancl_insert_max:
+  assumes "x \<notin> (r\<^sup>*) `` V" 
+  shows "(insert (x, y) r)\<^sup>+ `` V  = (r\<^sup>+) `` V" 
+  using assms
+  by (auto simp add: trancl_insert Un_Image L1)
+
+thm rtrancl_trancl_reflcl
+
+lemma Image_trancl_union_max:
+  assumes "finite B" "x \<notin> (r\<^sup>*) `` V" 
+  shows "((\<Union>y\<in>B. {(x, y)}) \<union> r)\<^sup>+ `` V = (r\<^sup>+) `` V" 
+  using assms
+  by (induction rule: finite.induct) 
+     (simp_all, metis Image_trancl_insert_max Un_Image rtrancl_trancl_reflcl)
+
+
+section \<open>Closedness: general definition and basic lemmas\<close>
+
+text \<open>Original general definition\<close>
+
+definition closed_general' :: "'a set \<Rightarrow> 'a rel \<Rightarrow> 'a set \<Rightarrow> bool" where
+  "closed_general' V r N \<longleftrightarrow> V = ((r\<^sup>*) `` V) - N"
+
+prop "V \<inter> N = {}"        \<comment> \<open>we can always assume this\<close>
+
+
+text \<open>Alternative def, equivalent under our conditions; probably easier to understand; 
+obviates need for some assumptions in lemmas below; also somewhat easier to work with?\<close>
+
+definition closed_general :: "'a set \<Rightarrow> 'a rel \<Rightarrow> 'a set \<Rightarrow> bool" where
+  "closed_general V r N \<longleftrightarrow> (r\<^sup>+) `` V \<subseteq> V \<union> N"
+
+lemma closed_generalI: "(r\<^sup>+) `` V \<subseteq> V \<union> N \<Longrightarrow> closed_general V r N"
+  by (simp add: closed_general_def)
+
+lemma closed_generalE [elim]: 
+  "\<lbrakk> closed_general V r N; (r\<^sup>+) `` V \<subseteq> V \<union> N \<Longrightarrow> P \<rbrakk> \<Longrightarrow> P"
+  by (simp add: closed_general_def)
+
+lemma closed_general_equiv:
+  assumes "V \<inter> N = {}"
+  shows "closed_general V r N \<longleftrightarrow> closed_general' V r N"
+  using assms
+  by (unfold closed_general_def closed_general'_def rtrancl_trancl_reflcl) 
+     blast  \<comment> \<open>rest just by general set theory\<close>
+
+
+text \<open>Empty set, monotonicity, and unions; note that monotonicity holds in @{term N}, but it
+does not hold in @{term V}.\<close>
+
+lemma closed_general_empty [simp, intro!]: 
+  shows "closed_general {} r N"
+  by (auto simp add: closed_general_def)
+
+lemma closed_general_mono_N [elim]:
+  assumes "closed_general V r N" 
+  and "N \<subseteq> N'"
+  shows "closed_general V r N'"
   using assms
   by (auto simp add: closed_general_def)
 
-lemma union_closed_general':
-  assumes "closed_general vis\<^sub>1 r r_only"
-      and "closed_general vis\<^sub>2 r r_only"
-      and "r_only \<subseteq> r_only'"
-      and "(r_only' - r_only) \<inter> (vis\<^sub>1 \<union> vis\<^sub>2) = {}"
-      and "r \<subseteq> r'"
-      and "Domain (r' - r) \<subseteq> r_only' - r_only"
-      and "Range (r' - r) \<inter> (r_only' - r_only) = {}"
-    shows "closed_general (vis\<^sub>1 \<union> vis\<^sub>2) r' r_only'"
-  using assms
-  apply (auto simp add: closed_general_def) oops
-
-lemma visTx'_union_distr: "visTx' K (u\<^sub>1 \<union> u\<^sub>2) = visTx' K u\<^sub>1 \<union> visTx' K u\<^sub>2"
-  by (auto simp add: visTx'_def)
-
-lemma visTx'_same_writers: "kvs_writers K' = kvs_writers K \<Longrightarrow> visTx' K' u = visTx' K u"
-  by (simp add: visTx'_def)
-
-lemma union_closed':
-  assumes "closed' K u\<^sub>1 r"
-    and "closed' K u\<^sub>2 r"
-    and "kvs_writers K' = kvs_writers K"
-    and "read_only_Txs K \<subseteq> read_only_Txs K'"
-    and "(read_only_Txs K' - read_only_Txs K) \<inter> (visTx' K' u\<^sub>1 \<union> visTx' K' u\<^sub>2) = {}"
-  shows "closed' K' (u\<^sub>1 \<union> u\<^sub>2) r"
-  using assms
-  by (auto simp add: closed'_generalize visTx'_union_distr visTx'_same_writers[of K']
-           intro!: union_closed_general)
-
-\<comment> \<open>insert new write\<close>
-lemma insert_t_closed_general:
-  assumes "closed_general vis r r_only"
-    and "t \<notin> vis"
-    and "t \<notin> r_only"
-    and "\<And>x. (t, x) \<in> r\<^sup>* \<Longrightarrow> x \<in> vis \<or> x \<in> r_only \<or> x = t"
-  shows "closed_general (insert t vis) r r_only"
+lemma closed_general_set_union_closed:   
+  assumes "closed_general V\<^sub>1 r N\<^sub>1"
+      and "closed_general V\<^sub>2 r N\<^sub>2"
+      and "V = V\<^sub>1 \<union> V\<^sub>2"
+      and "N\<^sub>1 \<union> N\<^sub>2 \<subseteq> V \<union> N"
+  shows "closed_general V r N"
   using assms
   by (auto simp add: closed_general_def)
 
-lemma visTx'_new_writer: "kvs_writers K' = insert t (kvs_writers K) \<Longrightarrow>
-  snd ` t_wr_deps = {t} \<Longrightarrow> visTx' K' (u \<union> t_wr_deps) = insert t (visTx' K u)"
-  by (auto simp add: visTx'_def)
-
-lemma insert_wr_t_closed':
-  assumes "closed' K u r"
-    and "t \<notin> visTx' K u"
-    and "\<And>x. (t, x) \<in> (r^-1)\<^sup>* \<Longrightarrow> x \<in> visTx' K u \<or> x \<in> read_only_Txs K \<or> x = t"
-    and "read_only_Txs K' = read_only_Txs K"
-    and "kvs_writers K' = insert t (kvs_writers K)"
-    and "snd ` t_wr_deps = {t}"
-  shows "closed' K' (u \<union> t_wr_deps) r"
+lemma closed_general_set_Union_closed:   
+  assumes "finite I"
+      and "\<And>i. i \<in> I \<Longrightarrow> closed_general (V i) r (N i)"
+      and "V' = (\<Union>i\<in>I. V i)"
+      and "(\<Union>i\<in>I. N i) \<subseteq> V' \<union> N'"
+  shows "closed_general V' r N'"
   using assms
-  apply (auto simp add: closed'_generalize visTx'_new_writer intro!: insert_t_closed_general)
-  by (metis insert_disjoint(2) inter_write_read_only)
+  apply (induction arbitrary: N' V' rule: finite.induct)
+   apply simp_all
+  by (rule closed_general_set_union_closed[where 
+             V\<^sub>1="V i" and V\<^sub>2="\<Union> (V ` I)" and N\<^sub>1="N i" and N\<^sub>2="\<Union> (N ` I)" for i I]) 
+     (auto) 
 
-\<comment> \<open>insert (k, t) in version's deps - used in get_ctx\<close>
-lemma visTx'_observes_t:
-  "t \<in> kvs_writers K \<Longrightarrow> visTx' K (insert (k, t) deps) = insert t (visTx' K deps)"
-  by (simp add: visTx'_def)
+text \<open>Extending the relation\<close>
 
-lemma insert_kt_to_deps_closed':
-  assumes "closed' K deps r"
-    and "t \<in> kvs_writers K"
-    and "t \<notin> visTx' K deps"
-    and "\<And>x. (t, x) \<in> (r^-1)\<^sup>* \<Longrightarrow> x \<in> visTx' K deps \<or> x \<in> read_only_Txs K \<or> x = t"
-  shows "closed' K (insert (k, t) deps) r"
+lemma closed_general_insert_rel_max:
+  assumes "closed_general V r N" 
+  and "r' = insert (x, y) r" 
+  and "x \<notin> (r\<^sup>*) `` V"                   \<comment> \<open>implies @{prop "x \<notin> V"} and @{prop "x \<notin> r``V"}\<close>
+  shows "closed_general V r' N"
   using assms
-  apply (auto simp add: closed'_generalize visTx'_observes_t intro!: insert_t_closed_general)
-  by (metis disjoint_insert(2) insert_absorb inter_write_read_only)
+  by (auto simp add: closed_general_def Image_trancl_insert_max)
 
-\<comment> \<open>concrete read_done closedness\<close>
+lemma closed_general_extend_rel_max:    \<comment> \<open>generalizes previous lemma\<close>
+  assumes "closed_general V r N" 
+  and "r' = (\<Union>y\<in>Y. {(x, y)}) \<union> r" 
+  and "x \<notin> (r\<^sup>*) `` V" 
+  and "finite Y"
+  shows "closed_general V r' N"
+  using assms
+  by (auto simp add: closed_general_def Image_trancl_union_max)
 
-lemma read_done_ctx_closed:
-  assumes "closed' (kvs_of_s s) (cl_ctx (cls s cl)) (R_CC (kvs_of_s s))"
-  shows "closed' (kvs_of_s s') (cl_ctx (cls s cl) \<union> get_ctx s kvt_map) (R_CC (kvs_of_s s'))"
-  oops (* not the same r !!!*)
+
+text  \<open>all at once ;-)\<close>
+
+lemma closed_general_union_V_extend_N_extend_rel:
+  assumes "closed_general V\<^sub>1 r N\<^sub>1"
+      and "closed_general V\<^sub>2 r N\<^sub>2"
+      and "V = V\<^sub>1 \<union> V\<^sub>2"
+      and "N\<^sub>1 \<union> N\<^sub>2 \<subseteq> V \<union> N"
+      and "x \<notin> (r\<^sup>*) `` V"
+      and "r' = (\<Union>y\<in>Y. {(x, y)}) \<union> r"
+      and "finite Y"
+    shows "closed_general V r' N"         \<comment> \<open>r changes as well!\<close>
+  using assms
+  by (auto intro: closed_general_set_union_closed[THEN closed_general_extend_rel_max])
+
+
+text \<open>
+  Q: Sufficent conditions to satisfy premise @{prop "x \<notin> (r\<^sup>*) `` V"} in the two previous lemmas?
+  In lemma below, first premise below does not necessarily hold for SO!
+\<close>
+lemma "\<lbrakk> x \<notin> Range r; x \<notin> V \<rbrakk> \<Longrightarrow> x \<notin> (r\<^sup>*) `` V"
+  by (metis ImageE Range_iff rtranclE)
+
+
+text \<open>Implications between closedness for different relations\<close>
+
+lemma closed_general_hierarchy:
+  assumes "closed_general V r N"
+  and "r'\<^sup>+ `` V \<subseteq> r\<^sup>+ `` V"
+  shows "closed_general V r' N"
+  using assms
+  by (simp add: closed_general_def)
+
+lemma closed_general_anti_mono:
+  assumes "closed_general V r N"
+  and "r' \<subseteq> r"
+  shows "closed_general V r' N"
+  using assms
+  by (auto elim!: closed_general_hierarchy elim: trancl_mono intro: Image_mono)
+
+text \<open>
+Q: Does the implication of closedness for different R_ET relations imply an ordering of 
+isolation guarantees? Not sure, since the execution test includes an initial view extension, 
+which need not be the same for different ETs to satisfy their respective commit conditions.
+\<close>
 
 end
